theories/tree_borrows/tree.v
@@ -3,9 +3,6 @@ From iris.prelude Require Import options.
 
 Implicit Type (V W X Y:Type).
 
-Definition app X : Type := X -> option X.
-Definition Tprop X : Type := X -> Prop.
-
 (** General Preliminaries *)
 
 #[global]
@@ -85,29 +82,29 @@ Definition join_nodes {X}
     Some $ branch data sibling child
   end.
 
-Definition every_subtree {X} (prop:Tprop (tbranch X)) (tr:tree X)
+Definition every_subtree {X} (prop:tbranch X -> Prop) (tr:tree X)
   := fold_subtrees True (fun sub lt rt => prop sub /\ lt /\ rt) tr.
 Global Instance every_subtree_dec {X} prop (tr:tree X) : (forall x, Decision (prop x)) -> Decision (every_subtree prop tr).
 Proof. intro. induction tr; solve_decision. Defined.
 
-Definition exists_subtree {X} (prop:Tprop (tbranch X)) (tr:tree X)
+Definition exists_subtree {X} (prop:tbranch X -> Prop) (tr:tree X)
   := fold_subtrees False (fun sub lt rt => prop sub \/ lt \/ rt) tr.
 Global Instance exists_subtree_dec {X} prop (tr:tree X) : (forall x, Decision (prop x)) -> Decision (exists_subtree prop tr).
 Proof. intro. induction tr; solve_decision. Defined.
 
-Definition every_node {X} (prop:Tprop X) (tr:tree X) := fold_nodes True (fun data lt rt => prop data /\ lt /\ rt) tr.
+Definition every_node {X} (prop:X -> Prop) (tr:tree X) := fold_nodes True (fun data lt rt => prop data /\ lt /\ rt) tr.
 Global Instance every_node_dec {X} prop (tr:tree X) : (forall x, Decision (prop x)) -> Decision (every_node prop tr).
 Proof. intro. induction tr; solve_decision. Defined.
 
-Definition exists_node {X} (prop:Tprop X) (tr:tree X) := fold_nodes False (fun data lt rt => prop data \/ lt \/ rt) tr.
+Definition exists_node {X} (prop:X -> Prop) (tr:tree X) := fold_nodes False (fun data lt rt => prop data \/ lt \/ rt) tr.
 Global Instance exists_node_dec {X} prop (tr:tree X) : (forall x, Decision (prop x)) -> Decision (exists_node prop tr).
 Proof. intro. induction tr; solve_decision. Defined.
 
 Definition count_nodes {X} (prop:X -> bool) :=
   fold_nodes 0 (fun data lt rt => (if prop data then 1 else 0) + lt + rt).
 
-Definition exists_strict_child {X} (prop:Tprop X)
-  : Tprop (tbranch X) := fun '(_, _, child) => exists_node prop child.
+Definition exists_strict_child {X} (prop:X -> Prop)
+  : tbranch X -> Prop := fun '(_, _, child) => exists_node prop child.
 Global Instance exists_strict_child_dec {X} prop (tr:tbranch X) :
   (forall u, Decision (prop u)) -> Decision (exists_strict_child prop tr).
 Proof. intro. solve_decision. Defined.
@@ -117,7 +114,7 @@ Definition empty_children {X} (tr:tbranch X)
   let '(_, _, children) := tr in
   children = empty.
 
-Definition insert_child_at {X} (tr:tree X) (ins:X) (search:Tprop X) {search_dec:forall x, Decision (search x)} : tree X :=
+Definition insert_child_at {X} (tr:tree X) (ins:X) (search:X -> Prop) {search_dec:forall x, Decision (search x)} : tree X :=
   (fix aux tr : tree X :=
     match tr with
     | empty => empty
@@ -142,7 +139,7 @@ Definition exists_sibling {X} (prop:X -> Prop) :=
 Global Instance exists_sibling_dec {X} prop (tr:tree X) : (forall x, Decision (prop x)) -> Decision (exists_sibling prop tr).
 Proof. intro. induction tr; solve_decision. Defined.
 Definition exists_immediate_child {X} (prop:X -> Prop)
-  : Tprop (tbranch X) := fun '(_, _, child) => exists_sibling prop child.
+  : tbranch X -> Prop := fun '(_, _, child) => exists_sibling prop child.
 Global Instance exists_immediate_child_dec {X} prop (tr:tbranch X) :
   (forall u, Decision (prop u)) -> Decision (exists_immediate_child prop tr).
 Proof. intro. solve_decision. Defined.
