theories/tree_borrows/trees_equal_endcall_law.v
@@ -454,7 +454,13 @@ Proof.
   intros l. specialize (Hutc l) as (Hproteq&Hutc).
   split; first done.
 
-  inversion Hutc as [x1 x2 Hlu|ini im confl1 confl2 (cc&Hcc&Hccact) Hpc1 Hpc2 Heqi1 Heqi2|ini im confl1 confl2 Hnprot|]; simplify_eq.
+  inversion Hutc as [
+    x1 x2 Hlu
+    |ini im confl1 confl2 (cc&Hcc&Hccact) Hpc1 Hpc2 Heqi1 Heqi2
+    |ini im confl1 confl2 Hnprot
+    |
+    |
+  ]; simplify_eq.
   - econstructor 1.
   - destruct (decide (cc = cid)) as [<-|Hne].
     + econstructor 3. intros (cc'&Hcc'&Hccact').
@@ -509,7 +515,9 @@ Proof.
     + eapply disabled_in_practice_cids_mono; last eassumption. set_solver.
     + assumption.
     + eapply protector_is_inactive_cids_mono; last eassumption. set_solver.
-Qed.
+  - econstructor 5.
+    all: admit.
+Admitted.
 
 Lemma trees_equal_remove_call C trs1' trs2' trs1 trs2 cid :
   wf_trees trs1 → wf_trees trs2 → each_tree_parents_more_init trs1 → each_tree_parents_more_init trs2 →
